BpmnSemantics/SemanticProcess.lean
@@ -7,6 +7,7 @@ import BpmnSemantics.SemanticProcess.ProgramStructuralValidation
 import BpmnSemantics.SemanticProcess.DefinitionBindingValidation
 import BpmnSemantics.SemanticProcess.ErrorDefinition
 import BpmnSemantics.SemanticProcess.Data
+import BpmnSemantics.SemanticProcess.ScopeCompletion
 import BpmnSemantics.SemanticProcess.Transition
 import BpmnSemantics.SemanticProcess.BoundedTask
 import BpmnSemantics.SemanticProcess.EventBasedGateway
